src/model/Promises.v
@@ -9,84 +9,20 @@ From PromisingLib Require Import Loc.
 From PromisingLib Require Import Language.
 From PromisingLib Require Import Event.
 
-Require Import Time.
+Require Import BoolMap.
 
 Set Implicit Arguments.
 
 
 Module Promises.
-  Definition t :=  Loc.t -> bool.
-
-  Definition bot: t := fun _ => false.
-
-  Definition le (lhs rhs: t): Prop :=
-    forall loc (LHS: lhs loc = true), rhs loc = true.
-
-  Global Program Instance le_PreOrder: PreOrder le.
-  Next Obligation.
-    ii. auto.
-  Qed.
-  Next Obligation.
-    ii. auto.
-  Qed.
-
-  Lemma antisym l r
-        (LR: le l r)
-        (RL: le r l):
-    l = r.
-  Proof.
-    extensionality loc.
-    specialize (LR loc). specialize (RL loc).
-    destruct (l loc) eqn:L, (r loc) eqn:R; eauto.
-    exploit LR; eauto.
-  Qed.
-
-  Lemma bot_spec prm: le bot prm.
-  Proof.
-    ii. ss.
-  Qed.
-
-  Definition disjoint (x y: t): Prop :=
-    forall loc (GET1: x loc = true) (GET2: y loc = true), False.
-
-  Global Program Instance disjoint_Symmetric: Symmetric disjoint.
-  Next Obligation.
-    ii. eauto.
-  Qed.
-
-  Lemma bot_disjoint prm: disjoint bot prm.
-  Proof.
-    ii. ss.
-  Qed.
-
-  Definition finite (prm: t): Prop :=
-    exists dom,
-    forall loc (GET: prm loc = true),
-      List.In loc dom.
-
-  Lemma bot_finite: finite bot.
-  Proof.
-    exists []. ss.
-  Qed.
-
-  
-  Variant add (prm1: t) (loc: Loc.t) (prm2: t): Prop :=
-  | add_intro
-      (GET: prm1 loc = false)
-      (PRM2: prm2 = LocFun.add loc true prm1)
-  .
-
-  Variant remove (prm1: t) (loc: Loc.t) (prm2: t): Prop :=
-  | remove_intro
-      (GET: prm1 loc = true)
-      (PRM2: prm2 = LocFun.add loc false prm1)
-  .
+  Import BoolMap.
 
   Variant promise (prm1 gprm1: t) (loc: Loc.t) (prm2 gprm2: t): Prop :=
   | promise_intro
       (ADD: add prm1 loc prm2)
       (GADD: add gprm1 loc gprm2)
   .
+  #[global] Hint Constructors promise: core.
 
   Variant fulfill (prm1 gprm1: t) (loc: Loc.t) (ord: Ordering.t) (prm2 gprm2: t): Prop :=
   | fulfill_refl
@@ -97,84 +33,8 @@ Module Promises.
       (REMOVE: remove prm1 loc prm2)
       (GREMOVE: remove gprm1 loc gprm2)
   .
+  #[global] Hint Constructors fulfill: core.
 
-
-  Lemma add_o
-        prm2 prm1 loc l
-        (ADD: add prm1 loc prm2):
-    prm2 l = if Loc.eq_dec l loc then true else prm1 l.
-  Proof.
-    inv ADD. unfold LocFun.add. ss.
-  Qed.
-
-  Lemma add_get0
-        prm1 loc prm2
-        (ADD: add prm1 loc prm2):
-    (<<GET1: prm1 loc = false>>) /\
-    (<<GET2: prm2 loc = true>>).
-  Proof.
-    inv ADD. split; ss.
-    unfold LocFun.add. condtac; ss.
-  Qed.
-
-  Lemma add_get1
-        prm1 loc prm2 l
-        (ADD: add prm1 loc prm2)
-        (GET: prm1 l = true):
-    prm2 l = true.
-  Proof.
-    inv ADD. unfold LocFun.add. condtac; ss.
-  Qed.
-
-  Lemma add_finite
-        prm1 loc prm2
-        (ADD: add prm1 loc prm2)
-        (FINITE: finite prm1):
-    finite prm2.
-  Proof.
-    inv ADD. inv FINITE.
-    exists (loc :: x). unfold LocFun.add. intro.
-    condtac; ss; eauto.
-  Qed.
-
-  Lemma remove_o
-        prm2 prm1 loc l
-        (REMOVE: remove prm1 loc prm2):
-    prm2 l = if Loc.eq_dec l loc then false else prm1 l.
-  Proof.
-    inv REMOVE. unfold LocFun.add. ss.
-  Qed.
-
-  Lemma remove_get0
-        prm1 loc prm2
-        (REMOVE: remove prm1 loc prm2):
-    (<<GET1: prm1 loc = true>>) /\
-    (<<GET2: prm2 loc = false>>).
-  Proof.
-    inv REMOVE. split; ss.
-    unfold LocFun.add. condtac; ss.
-  Qed.
-
-  Lemma remove_get1
-        prm1 loc prm2 l
-        (REMOVE: remove prm1 loc prm2)
-        (GET: prm1 l = true):
-    (<<LOC: l = loc>>) \/
-    (<<GET2: prm2 l = true>>).
-  Proof.
-    inv REMOVE. unfold LocFun.add. condtac; auto.
-  Qed.
-
-  Lemma remove_finite
-        prm1 loc prm2
-        (REMOVE: remove prm1 loc prm2)
-        (FINITE: finite prm1):
-    finite prm2.
-  Proof.
-    inv REMOVE. inv FINITE.
-    exists x. unfold LocFun.add. intro.
-    condtac; ss; eauto.
-  Qed.
 
   Lemma promise_le
         prm1 gprm1 loc prm2 gprm2
