src/model/Reserves.v
@@ -9,266 +9,45 @@ From PromisingLib Require Import Loc.
 From PromisingLib Require Import Language.
 From PromisingLib Require Import Event.
 
-Require Import Time.
+Require Import BoolMap.
 
 Set Implicit Arguments.
 
 
-(* TODO: move to promising-lib *)
-
-Variant option_le (A: Type) (le: A -> A -> Prop): forall (lhs rhs: option A), Prop :=
-| option_le_None
-    rhs:
-  option_le le None rhs
-| option_le_Some
-    lhs rhs
-    (LE: le lhs rhs):
-  option_le le (Some lhs) (Some rhs)
-.
-#[export] Hint Constructors option_le: core.
-
-#[export] Program Instance option_le_PreOrder A (le: A -> A -> Prop) `{PreOrder A le}:
-  PreOrder (option_le le).
-Next Obligation.
-  ii. destruct x; eauto. econs. refl.
-Qed.
-Next Obligation.
-  ii. inv H0; inv H1; eauto. econs. etrans; eauto.
-Qed.
-
-Definition option_join (A: Type) (join: A -> A -> A) (lhs rhs: option A): option A :=
-  match lhs, rhs with
-  | None, _ => rhs
-  | _, None => lhs
-  | Some l, Some r => Some (join l r)
-  end.
-
-Lemma option_join_comm
-      A (join: A -> A -> A)
-      (COMM: forall x y, join x y = join y x):
-  forall x y, option_join join x y = option_join join y x.
-Proof.
-  i. destruct x, y; ss. f_equal. auto.
-Qed.
-
-Lemma option_join_assoc
-      A (join: A -> A -> A)
-      (ASSOC: forall x y z, join (join x y) z = join x (join y z)):
-  forall x y z,
-    option_join join (option_join join x y) z =
-    option_join join x (option_join join y z).
-Proof.
-  i. destruct x, y, z; ss. f_equal. auto.
-Qed.
-
-Lemma option_join_spec
-      A (le: A -> A -> Prop) (join: A -> A -> A)
-      (SPEC: forall x y o, le x o -> le y o -> le (join x y) o):
-  forall x y o,
-    option_le le x o -> option_le le y o ->
-    option_le le (option_join join x y) o.
-Proof.
-  i. inv H; inv H0; econs; eauto.
-Qed.
-
-
 Module Reserves.
-  Definition t := Loc.t -> option Time.t.
+  Import BoolMap.
 
-  Definition eq := @eq t.
-
-  Definition incl (lhs rhs: t): Prop :=
-    forall loc ts (LHS: lhs loc = Some ts),
-      rhs loc = Some ts.
-
-  Lemma incl_antisym l r
-        (LR: incl l r)
-        (RL: incl r l):
-    l = r.
-  Proof.
-    extensionality loc.
-    specialize (LR loc). specialize (RL loc).
-    destruct (l loc) eqn:L, (r loc) eqn:R; eauto.
-    exploit LR; eauto.
-  Qed.
-
-  Global Program Instance incl_PreOrder: PreOrder incl.
-  Next Obligation. ii. ss. Qed.
-  Next Obligation. ii. eauto. Qed.
-  #[global] Hint Resolve incl_PreOrder_obligation_2: core.
-
-  Definition le (lhs rhs: t): Prop :=
-    forall loc, option_le Time.le (lhs loc) (rhs loc).
-
-  Lemma le_antisym l r
-        (LR: le l r)
-        (RL: le r l):
-    l = r.
-  Proof.
-    extensionality loc.
-    specialize (LR loc). specialize (RL loc).
-    inv LR; inv RL; try congr.
-    rewrite <- H0, <- H in *. clarify.
-    f_equal. apply TimeFacts.antisym; ss.
-  Qed.
-
-  Definition disjoint (x y: t): Prop :=
-    forall loc ts1 ts2
-      (GET1: x loc = Some ts1)
-      (GET2: y loc = Some ts2),
-      False.
-
-  Global Program Instance disjoint_Symmetric: Symmetric disjoint.
-  Next Obligation.
-    ii. eauto.
-  Qed.
-
-  Definition finite (rsv: t): Prop :=
-    exists dom,
-    forall loc ts (GET: rsv loc = Some ts),
-      List.In loc dom.
-
-  Definition bot: t := fun _ => None.
-
-  Lemma bot_incl (rsv: t): incl bot rsv.
-  Proof.
-    ii. ss.
-  Qed.
-
-  Lemma bot_le (rsv: t): le bot rsv.
-  Proof.
-    ii. econs.
-  Qed.
-
-  Lemma bot_disjoint prom: disjoint bot prom.
-  Proof.
-    ii. ss.
-  Qed.
-
-  Lemma bot_finite: finite bot.
-  Proof.
-    exists []. ss.
-  Qed.
-
-  
-  Variant add (rsv1: t) (loc: Loc.t) (ts: Time.t) (rsv2: t): Prop :=
-  | add_intro
-      (GET: rsv1 loc = None)
-      (RSV2: rsv2 = LocFun.add loc (Some ts) rsv1)
-  .
-
-  Variant remove (rsv1: t) (loc: Loc.t) (ts: Time.t) (rsv2: t): Prop :=
-  | remove_intro
-      (GET: rsv1 loc = Some ts)
-      (RSV2: rsv2 = LocFun.add loc None rsv1)
-  .
-
-  Variant reserve (rsv1 grsv1: t) (loc: Loc.t) (ts: Time.t) (rsv2 grsv2: t): Prop :=
+  Variant reserve (rsv1 grsv1: t) (loc: Loc.t) (rsv2 grsv2: t): Prop :=
   | reserve_intro
-      (ADD: add rsv1 loc ts rsv2)
-      (GADD: add grsv1 loc ts grsv2)
+      (ADD: add rsv1 loc rsv2)
+      (GADD: add grsv1 loc grsv2)
   .
+  #[global] Hint Constructors reserve: core.
 
-  Variant cancel (rsv1 grsv1: t) (loc: Loc.t) (ts: Time.t) (rsv2 grsv2: t): Prop :=
+  Variant cancel (rsv1 grsv1: t) (loc: Loc.t) (rsv2 grsv2: t): Prop :=
   | cancel_intro
-      (REMOVE: remove rsv1 loc ts rsv2)
-      (GREMOVE: remove grsv1 loc ts grsv2)
+      (REMOVE: remove rsv1 loc rsv2)
+      (GREMOVE: remove grsv1 loc grsv2)
   .
+  #[global] Hint Constructors cancel: core.
 
 
-  Lemma add_o
-        rsv2 rsv1 loc ts l
-        (ADD: add rsv1 loc ts rsv2):
-    rsv2 l = if Loc.eq_dec l loc then Some ts else rsv1 l.
-  Proof.
-    inv ADD. unfold LocFun.add. ss.
-  Qed.
-
-  Lemma add_get0
-        rsv1 loc ts rsv2
-        (ADD: add rsv1 loc ts rsv2):
-    (<<GET1: rsv1 loc = None>>) /\
-    (<<GET2: rsv2 loc = Some ts>>).
-  Proof.
-    inv ADD. split; ss.
-    unfold LocFun.add. condtac; ss.
-  Qed.
-
-  Lemma add_get1
-        rsv1 loc ts rsv2 l ts'
-        (ADD: add rsv1 loc ts rsv2)
-        (GET: rsv1 l = Some ts'):
-    rsv2 l = Some ts'.
-  Proof.
-    inv ADD. unfold LocFun.add. condtac; ss. subst. congr.
-  Qed.
-
-  Lemma add_finite
-        rsv1 loc ts rsv2
-        (ADD: add rsv1 loc ts rsv2)
-        (FINITE: finite rsv1):
-    finite rsv2.
-  Proof.
-    inv ADD. inv FINITE.
-    exists (loc :: x). unfold LocFun.add. intro.
-    condtac; ss; eauto.
-  Qed.
-
-  Lemma remove_o
-        rsv2 rsv1 loc ts l
-        (REMOVE: remove rsv1 loc ts rsv2):
-    rsv2 l = if Loc.eq_dec l loc then None else rsv1 l.
-  Proof.
-    inv REMOVE. unfold LocFun.add. ss.
-  Qed.
-
-  Lemma remove_get0
-        rsv1 loc ts rsv2
-        (REMOVE: remove rsv1 loc ts rsv2):
-    (<<GET1: rsv1 loc = Some ts>>) /\
-    (<<GET2: rsv2 loc = None>>).
-  Proof.
-    inv REMOVE. split; ss.
-    unfold LocFun.add. condtac; ss.
-  Qed.
-
-  Lemma remove_get1
-        rsv1 loc ts rsv2 l ts'
-        (REMOVE: remove rsv1 loc ts rsv2)
-        (GET: rsv1 l = Some ts'):
-    (<<LOC: l = loc>>) \/
-    (<<GET2: rsv2 l = Some ts'>>).
-  Proof.
-    inv REMOVE. unfold LocFun.add. condtac; auto.
-  Qed.
-
-  Lemma remove_finite
-        rsv1 loc ts rsv2
-        (REMOVE: remove rsv1 loc ts rsv2)
-        (FINITE: finite rsv1):
-    finite rsv2.
-  Proof.
-    inv REMOVE. inv FINITE.
-    exists x. unfold LocFun.add. intro.
-    condtac; ss; eauto.
-  Qed.
-
-  Lemma reserve_incl
-        rsv1 grsv1 loc ts rsv2 grsv2
-        (RESERVE: reserve rsv1 grsv1 loc ts rsv2 grsv2)
-        (LE1: incl rsv1 grsv1):
-    incl rsv2 grsv2.
+  Lemma reserve_le
+        rsv1 grsv1 loc rsv2 grsv2
+        (RESERVE: reserve rsv1 grsv1 loc rsv2 grsv2)
+        (LE1: le rsv1 grsv1):
+    le rsv2 grsv2.
   Proof.
     ii. revert LHS.
     inv RESERVE. inv ADD. inv GADD.
     unfold LocFun.add. condtac; ss. eauto.
   Qed.
 
-  Lemma cancel_incl
-        rsv1 grsv1 loc ts rsv2 grsv2
-        (CANCEL: cancel rsv1 grsv1 loc ts rsv2 grsv2)
-        (LE1: incl rsv1 grsv1):
-    incl rsv2 grsv2.
+  Lemma cancel_le
+        rsv1 grsv1 loc rsv2 grsv2
+        (CANCEL: cancel rsv1 grsv1 loc rsv2 grsv2)
+        (LE1: le rsv1 grsv1):
+    le rsv2 grsv2.
   Proof.
     ii. revert LHS.
     inv CANCEL. inv REMOVE. inv GREMOVE.
@@ -276,41 +55,38 @@ Module Reserves.
   Qed.
 
   Lemma reserve_disjoint
-        rsv1 grsv1 loc ts rsv2 grsv2
+        rsv1 grsv1 loc rsv2 grsv2
         ctx
-        (RESERVE: reserve rsv1 grsv1 loc ts rsv2 grsv2)
-        (LE_CTX: incl ctx grsv1)
+        (RESERVE: reserve rsv1 grsv1 loc rsv2 grsv2)
+        (LE_CTX: le ctx grsv1)
         (DISJOINT: disjoint rsv1 ctx):
     (<<DISJOINT: disjoint rsv2 ctx>>) /\
-    (<<LE_CTX: incl ctx grsv2>>).
+    (<<LE_CTX: le ctx grsv2>>).
   Proof.
     inv RESERVE. inv ADD. inv GADD. splits; ii.
     - revert GET1. unfold LocFun.add.
-      condtac; ss; subst; eauto. i. clarify.
-      exploit LE_CTX; eauto. i. congr.
-    - unfold LocFun.add. condtac; ss; eauto. clarify.
-      exploit LE_CTX; eauto. i. congr.
+      condtac; ss; subst; eauto.
+    - unfold LocFun.add. condtac; ss; eauto.
   Qed.
 
   Lemma cancel_disjoint
-        rsv1 grsv1 loc ts rsv2 grsv2
+        rsv1 grsv1 loc rsv2 grsv2
         ctx
-        (CANCEL: cancel rsv1 grsv1 loc ts rsv2 grsv2)
-        (LE_CTX: incl ctx grsv1)
+        (CANCEL: cancel rsv1 grsv1 loc rsv2 grsv2)
+        (LE_CTX: le ctx grsv1)
         (DISJOINT: disjoint rsv1 ctx):
     (<<DISJOINT: disjoint rsv2 ctx>>) /\
-    (<<LE_CTX: incl ctx grsv2>>).
+    (<<LE_CTX: le ctx grsv2>>).
   Proof.
     inv CANCEL. inv REMOVE. inv GREMOVE. splits; ii.
     - revert GET1. unfold LocFun.add.
       condtac; ss; subst; eauto.
     - unfold LocFun.add. condtac; ss; subst; eauto.
-      exploit DISJOINT; eauto. ss.
   Qed.
 
   Lemma reserve_finite
-        rsv1 grsv1 loc ts rsv2 grsv2
-        (RESERVE: reserve rsv1 grsv1 loc ts rsv2 grsv2)
+        rsv1 grsv1 loc rsv2 grsv2
+        (RESERVE: reserve rsv1 grsv1 loc rsv2 grsv2)
         (FINITE: finite rsv1):
     finite rsv2.
   Proof.
@@ -318,8 +94,8 @@ Module Reserves.
   Qed.
 
   Lemma cancel_finite
-        rsv1 grsv1 loc ts rsv2 grsv2
-        (CANCEL: cancel rsv1 grsv1 loc ts rsv2 grsv2)
+        rsv1 grsv1 loc rsv2 grsv2
+        (CANCEL: cancel rsv1 grsv1 loc rsv2 grsv2)
         (FINITE: finite rsv1):
     finite rsv2.
   Proof.
