src/model/BoolMap.v
@@ -1,0 +1,162 @@
+Require Import RelationClasses.
+
+From sflib Require Import sflib.
+
+From PromisingLib Require Import Axioms.
+From PromisingLib Require Import Basic.
+From PromisingLib Require Import DataStructure.
+From PromisingLib Require Import Loc.
+From PromisingLib Require Import Language.
+From PromisingLib Require Import Event.
+
+Set Implicit Arguments.
+
+
+Module BoolMap.
+  Definition t :=  Loc.t -> bool.
+
+  Definition bot: t := fun _ => false.
+
+  Definition le (lhs rhs: t): Prop :=
+    forall loc (LHS: lhs loc = true), rhs loc = true.
+
+  Global Program Instance le_PreOrder: PreOrder le.
+  Next Obligation.
+    ii. auto.
+  Qed.
+  Next Obligation.
+    ii. auto.
+  Qed.
+
+  Lemma antisym l r
+        (LR: le l r)
+        (RL: le r l):
+    l = r.
+  Proof.
+    extensionality loc.
+    specialize (LR loc). specialize (RL loc).
+    destruct (l loc) eqn:L, (r loc) eqn:R; eauto.
+    exploit LR; eauto.
+  Qed.
+
+  Lemma bot_spec bm: le bot bm.
+  Proof.
+    ii. ss.
+  Qed.
+
+  Definition disjoint (x y: t): Prop :=
+    forall loc (GET1: x loc = true) (GET2: y loc = true), False.
+
+  Global Program Instance disjoint_Symmetric: Symmetric disjoint.
+  Next Obligation.
+    ii. eauto.
+  Qed.
+
+  Lemma bot_disjoint bm: disjoint bot bm.
+  Proof.
+    ii. ss.
+  Qed.
+
+  Definition finite (bm: t): Prop :=
+    exists dom,
+    forall loc (GET: bm loc = true),
+      List.In loc dom.
+
+  Lemma bot_finite: finite bot.
+  Proof.
+    exists []. ss.
+  Qed.
+
+
+  Variant add (bm1: t) (loc: Loc.t) (bm2: t): Prop :=
+  | add_intro
+      (GET: bm1 loc = false)
+      (BM2: bm2 = LocFun.add loc true bm1)
+  .
+  #[global] Hint Constructors add: core.
+
+  Variant remove (bm1: t) (loc: Loc.t) (bm2: t): Prop :=
+  | remove_intro
+      (GET: bm1 loc = true)
+      (BM2: bm2 = LocFun.add loc false bm1)
+  .
+  #[global] Hint Constructors remove: core.
+
+
+  Lemma add_o
+        bm2 bm1 loc l
+        (ADD: add bm1 loc bm2):
+    bm2 l = if Loc.eq_dec l loc then true else bm1 l.
+  Proof.
+    inv ADD. unfold LocFun.add. ss.
+  Qed.
+
+  Lemma add_get0
+        bm1 loc bm2
+        (ADD: add bm1 loc bm2):
+    (<<GET1: bm1 loc = false>>) /\
+    (<<GET2: bm2 loc = true>>).
+  Proof.
+    inv ADD. split; ss.
+    unfold LocFun.add. condtac; ss.
+  Qed.
+
+  Lemma add_get1
+        bm1 loc bm2 l
+        (ADD: add bm1 loc bm2)
+        (GET: bm1 l = true):
+    bm2 l = true.
+  Proof.
+    inv ADD. unfold LocFun.add. condtac; ss.
+  Qed.
+
+  Lemma add_finite
+        bm1 loc bm2
+        (ADD: add bm1 loc bm2)
+        (FINITE: finite bm1):
+    finite bm2.
+  Proof.
+    inv ADD. inv FINITE.
+    exists (loc :: x). unfold LocFun.add. intro.
+    condtac; ss; eauto.
+  Qed.
+
+  Lemma remove_o
+        bm2 bm1 loc l
+        (REMOVE: remove bm1 loc bm2):
+    bm2 l = if Loc.eq_dec l loc then false else bm1 l.
+  Proof.
+    inv REMOVE. unfold LocFun.add. ss.
+  Qed.
+
+  Lemma remove_get0
+        bm1 loc bm2
+        (REMOVE: remove bm1 loc bm2):
+    (<<GET1: bm1 loc = true>>) /\
+    (<<GET2: bm2 loc = false>>).
+  Proof.
+    inv REMOVE. split; ss.
+    unfold LocFun.add. condtac; ss.
+  Qed.
+
+  Lemma remove_get1
+        bm1 loc bm2 l
+        (REMOVE: remove bm1 loc bm2)
+        (GET: bm1 l = true):
+    (<<LOC: l = loc>>) \/
+    (<<GET2: bm2 l = true>>).
+  Proof.
+    inv REMOVE. unfold LocFun.add. condtac; auto.
+  Qed.
+
+  Lemma remove_finite
+        bm1 loc bm2
+        (REMOVE: remove bm1 loc bm2)
+        (FINITE: finite bm1):
+    finite bm2.
+  Proof.
+    inv REMOVE. inv FINITE.
+    exists x. unfold LocFun.add. intro.
+    condtac; ss; eauto.
+  Qed.
+End BoolMap.
