src/model/Global.v
@@ -11,6 +11,7 @@ From PromisingLib Require Import Event.
 
 Require Import Time.
 Require Import View.
+Require Import BoolMap.
 Require Import Promises.
 Require Import Reserves.
 Require Import Cell.
@@ -22,17 +23,16 @@ Set Implicit Arguments.
 Module Global.
   Structure t := mk {
     sc: TimeMap.t;
-    promises: Promises.t;
-    reserves: Reserves.t;
+    promises: BoolMap.t;
+    reserves: BoolMap.t;
     memory: Memory.t;
   }.
 
-  Definition init := mk TimeMap.bot Promises.bot Reserves.bot Memory.init.
+  Definition init := mk TimeMap.bot BoolMap.bot BoolMap.bot Memory.init.
 
   Variant wf (gl: t): Prop :=
   | wf_intro
       (SC_CLOSED: Memory.closed_timemap (sc gl) (memory gl))
-      (RSV_CLOSED: Memory.closed_reserves (reserves gl) (memory gl))
       (MEM_CLOSED: Memory.closed (memory gl))
   .
 
@@ -42,23 +42,5 @@ Module Global.
     - apply Memory.closed_timemap_bot.
       apply Memory.init_closed.
     - apply Memory.init_closed.
-  Qed.
-
-  Definition max_reserves (rsv: Reserves.t) (gl: t): t :=
-    mk (sc gl)
-       (promises gl)
-       (Memory.max_reserves rsv (memory gl))
-       (memory gl).
-
-  Lemma max_reserves_wf
-        rsv gl
-        (CLOSED: Memory.closed_reserves rsv (memory gl))
-        (WF: wf gl):
-    wf (max_reserves rsv gl).
-  Proof.
-    destruct gl as [sc prm grsv mem]. inv WF. ss.
-    econs; eauto; ss.
-    eapply Memory.max_reserves_closed; eauto.
-    apply MEM_CLOSED.
   Qed.
 End Global.
